rocq-skylabs-brick/theories/lang/cpp/semantics/types.v
@@ -9,30 +9,28 @@ Require Export skylabs.prelude.option.
 Require Import skylabs.lang.cpp.syntax.
 Require Import skylabs.lang.cpp.semantics.genv.
 
+Fixpoint fundamental_size (t : type) : option N :=
+  match t with
+  | Tqualified _ t
+  | TLocInfo _ t => fundamental_size t
+  | Tchar_ sz => Some $ char_type.bytesN sz
+  | Tnum sz _ => Some $ int_rank.bytesN sz
+  | Tbool => Some 1%N
+  | _ => None
+  end.
+
 Definition GlobDecl_size_of (g : GlobDecl) : option N :=
   match g with
   | Gstruct s => Some s.(s_size)
   | Gunion u => Some u.(u_size)
-  | Genum t _ =>
-    match drop_qualifiers t with
-    | Tchar_ sz => Some $ char_type.bytesN sz
-    | Tnum sz _ => Some $ int_rank.bytesN sz
-    | Tbool => Some 1%N
-    | _ => None
-    end
+  | Genum t _ => fundamental_size t
   | _ => None
   end.
 Definition GlobDecl_align_of (g : GlobDecl) : option N :=
   match g with
   | Gstruct s => Some s.(s_alignment)
   | Gunion u => Some u.(u_alignment)
-  | Genum t _ =>
-    match drop_qualifiers t with
-    | Tchar_ sz => Some $ char_type.bytesN sz
-    | Tnum sz _ => Some $ int_rank.bytesN sz
-    | Tbool => Some 1%N
-    | _ => None
-    end
+  | Genum t _ => fundamental_size t
   | _ => None
   end.
 
@@ -43,15 +41,19 @@ Proof.
   do 2 case_match; subst; try contradiction; try constructor.
   case_bool_decide; subst; eauto. contradiction.
   case_bool_decide; subst; eauto. contradiction.
-  case_bool_decide; subst; eauto. case_match; constructor; eauto. contradiction.
+  case_bool_decide.
+  { subst. destruct (fundamental_size t0); constructor; eauto. }
+  { contradiction. }
 Qed.
 #[global] Instance proper_GlobDecl_align_of: Proper (GlobDecl_ler ==> Roption_leq eq) GlobDecl_align_of.
 Proof.
-  rewrite /GlobDecl_size_of/GlobDecl_ler/GlobDecl_le => x y Heq.
+  rewrite /GlobDecl_align_of/GlobDecl_ler/GlobDecl_le => x y Heq.
   do 2 case_match; subst; try contradiction; try constructor.
   case_bool_decide; subst; eauto. contradiction.
   case_bool_decide; subst; eauto. contradiction.
-  case_bool_decide; subst; eauto. simpl. case_match; constructor; eauto. contradiction.
+  case_bool_decide.
+  { subst. destruct (fundamental_size t0); constructor; eauto. }
+  { contradiction. }
 Qed.
 
 (** * sizeof *)
@@ -96,6 +98,7 @@ Fixpoint size_of (resolve : genv) (t : type) : option N :=
   | Tresult_call _ _
   | Tresult_member_call _ _ _
   | Tauto => None
+  | TLocInfo _ t => size_of resolve t
   end%N.
 
 (* [size_of] result can overflow: *)
@@ -274,9 +277,8 @@ Proof. by rewrite /SizeOf TCEq_eq=><-. Qed.
 
 Lemma size_of_to_heap_type g ty : size_of g (to_heap_type ty) = size_of g ty.
 Proof.
-  rewrite -(size_of_erase_qualifiers _ ty).
-  rewrite /to_heap_type.
-  by destruct (erase_qualifiers ty).
+  induction ty; simpl; auto. all: try by rewrite IHty.
+  by rewrite size_of_erase_qualifiers.
 Qed.
 
 (** [HasSize ty] means that C++ type [ty] has a defined size *)
@@ -447,6 +449,9 @@ Section with_genv.
     intros.
     rewrite -{1}align_of_erase_qualifiers. simpl. by rewrite align_of_erase_qualifiers.
   Qed.
+
+  Axiom align_of_loc_info : ∀ li t,
+      align_of (TLocInfo li t) = align_of t.
 
   Axiom Proper_align_of : Proper (genv_leq ==> eq ==> Roption_leq eq) (@align_of).
   #[global] Existing Instance Proper_align_of.
