rocq-skylabs-brick/theories/lang/cpp/semantics/cast_operator.v
@@ -25,8 +25,10 @@ Require Import skylabs.lang.cpp.semantics.cast.
   *)
 Notation Tptrdiff_t := Tlonglong (only parsing).
 
-Definition supported_float_type (ty : type) : option float_type.t :=
-  match drop_qualifiers ty with
+Fixpoint supported_float_type (ty : type) : option float_type.t :=
+  match ty with
+  | Tqualified _ ty
+  | TLocInfo _ ty => supported_float_type ty
   | Tfloat_ ft => if float_type.supported ft then Some ft else None
   | _ => None
   end.
