rocq-skylabs-brick/theories/lang/cpp/syntax/name_notation/printer.v
@@ -46,7 +46,7 @@ Section with_lang.
     Variable top : option PrimString.string.
 
     #[local] Open Scope monad_scope.
-    Definition printAN inst (an : atomic_name) : option PrimString.string :=
+    Fixpoint printAN inst (an : atomic_name) : option PrimString.string :=
       match an return option PrimString.string with
       | Nid id =>
           if bool_decide (id = "") then mfail else mret $ id ++ inst
@@ -81,6 +81,7 @@ Section with_lang.
       | Nfirst_decl n => mret $ "@" ++ n ++ inst
       | Nfirst_child n => mret $ "." ++ n ++ inst
       | Nunsupported_atomic note => mfail
+      | ANLocInfo _ an => printAN inst an
       end.
   End atomic_name.
 
@@ -89,6 +90,7 @@ Section with_lang.
     | Nglobal (Nid id) => Some id
     | Nscoped _ (Nid id) => Some id
     | Ninst nm _ => topName nm
+    | NLocInfo _ nm => topName nm
     | _ => None
     end.
 
@@ -164,11 +166,13 @@ Section with_lang.
           | Atemplate_param id =>
               mret $ "template " ++ id
           | Aunsupported note => mfail
+          | ALocInfo _ ta => printTA ta
           end
         in
         ((fun tas => angles $ sepBy ", " tas) <$> traverse printTA i) ≫= fun tas =>
         printN tas base
     | Nunsupported note => mfail
+    | NLocInfo _ nm => printN inst nm
     end
 
   with printT (is_arg : bool) (ty : type) : option PrimString.string :=
@@ -255,6 +259,7 @@ Section with_lang.
     | Tarch _ note => mfail
     | Tunsupported note => mfail
     | Tparam nm => mret $ "$" ++ nm
+    | TLocInfo _ ty => printT is_arg ty
     | _ => mfail
     end
 
@@ -277,6 +282,7 @@ Section with_lang.
     | Ebool b => mret $ if b then "true" else "false"
     | Enull => mret "nullptr"
     | Eparam b => mret $ "`" ++ b
+    | ELocInfo _ e => printE e
     | _ => mfail
     end.
 
