rocq-skylabs-brick/theories/lang/cpp/syntax/translation_unit.v
@@ -367,13 +367,14 @@ Module template_alias.
     | _ => None
     end.
 
-  Definition subst_expr (xs : env) (e : Expr) : Expr :=
+  Fixpoint subst_expr (xs : env) (e : Expr) : Expr :=
     match e with
     | Eparam id =>
         match lookup_value xs id with
         | Some e => e
         | None => e
         end
+    | ELocInfo li e => ELocInfo li (subst_expr xs e)
     | _ => e
     end.
 
@@ -387,6 +388,7 @@ Module template_alias.
     | Ndependent t => Ndependent' (subst_type xs t)
     | Nscoped n c => Nscoped (subst_name xs n) c
     | Nunsupported _ => n
+    | NLocInfo li n => NLocInfo li (subst_name xs n)
     end
 
   with subst_temp_arg (xs : env) (a : temp_arg) : temp_arg :=
@@ -401,6 +403,7 @@ Module template_alias.
         | None => a
         end
     | Aunsupported _ => a
+    | ALocInfo li a => ALocInfo li (subst_temp_arg xs a)
     end
 
   with subst_type (xs : env) (t : type) : type :=
@@ -450,6 +453,7 @@ Module template_alias.
     | Tmember_pointer n t => Tmember_pointer (subst_type xs n) (subst_type xs t)
     | Tdecltype e => Tdecltype (subst_expr xs e)
     | Texprtype e => Texprtype (subst_expr xs e)
+    | TLocInfo li t => TLocInfo li (subst_type xs t)
     end.
 
   Definition same_template_base (actual candidate : name) : option (list temp_arg) :=
@@ -550,24 +554,25 @@ Definition resolve_value (tu : translation_unit) (nm : name) : option name :=
     This classifies references as trivially destructible.
  *)
 Fixpoint is_trivially_destructible (tu : translation_unit) (ty : type) {struct ty} : bool :=
-  qual_norm (fun _ t =>
-               match t with
-               | Tref _ | Trv_ref _
-               | Tnum _ _ | Tchar_ _
-               | Tvoid | Tbool | Tptr _
-               | Tenum _
-               | Tmember_pointer _ _
-               | Tfloat_ _
-               | Tnullptr => true
-               | Tnamed nm =>
-                   match tu.(types) !! nm with
-                   | Some (Gunion u) => u.(u_trivially_destructible)
-                   | Some (Gstruct s) => s.(s_trivially_destructible)
-                   | _ => false
-                   end
-               | Tarray ety _ => is_trivially_destructible tu ety
-               | _ => false
-               end) ty.
+  match ty with
+  | Tqualified _ ty
+  | TLocInfo _ ty => is_trivially_destructible tu ty
+  | Tref _ | Trv_ref _
+  | Tnum _ _ | Tchar_ _
+  | Tvoid | Tbool | Tptr _
+  | Tenum _
+  | Tmember_pointer _ _
+  | Tfloat_ _
+  | Tnullptr => true
+  | Tnamed nm =>
+      match tu.(types) !! nm with
+      | Some (Gunion u) => u.(u_trivially_destructible)
+      | Some (Gstruct s) => s.(s_trivially_destructible)
+      | _ => false
+      end
+  | Tarray ety _ => is_trivially_destructible tu ety
+  | _ => false
+  end.
 
 (**
 TODO: The following work on complete types seems misplaced.
@@ -576,7 +581,8 @@ Fixpoint ref_to_type (t : type) : option type :=
   match t with
   | Tref t
   | Trv_ref t => Some t
-  | Tqualified _ t => ref_to_type t
+  | Tqualified _ t
+  | TLocInfo _ t => ref_to_type t
   | _ => None
   end.
 
@@ -630,6 +636,8 @@ Section with_type_table.
   | complete_bool : complete_basic_type Tbool
   | complete_nullptr : complete_basic_type Tnullptr
   | complete_char c : complete_basic_type (Tchar_ c)
+  | complete_basic_loc_info {li t} (_ : complete_basic_type t) :
+    complete_basic_type (TLocInfo li t)
 
   (* t can in turn be a pointer type *)
   | complete_ptr {t} : complete_pointee_type t -> complete_basic_type (Tptr t)
@@ -640,6 +648,8 @@ Section with_type_table.
   with complete_pointee_type : type -> Prop :=
   | complete_pt_qualified {q t} (_ : complete_pointee_type t)
     : complete_pointee_type (Tqualified q t)
+  | complete_pt_loc_info {li t} (_ : complete_pointee_type t)
+    : complete_pointee_type (TLocInfo li t)
   (*
     Pointers to array are only legal if the array is complete, at least
     in C, since they cannot actually be indexed or created.
@@ -685,6 +695,8 @@ Section with_type_table.
   with complete_type : type -> Prop :=
   | complete_qualified {q t} (_ : complete_type t)
     : complete_type (Tqualified q t)
+  | complete_loc_info {li t} (_ : complete_type t)
+    : complete_type (TLocInfo li t)
   (* Reference types. This setup forbids references to references. *)
   | complete_ref {t} : complete_pointee_type t -> complete_type (Tref t)
   | complete_rv_ref {t} : complete_pointee_type t -> complete_type (Trv_ref t)
@@ -723,6 +735,8 @@ Section with_type_table.
   with wellscoped_type : type -> Prop :=
   | wellscoped_qualified {q t} (_ : wellscoped_type t)
     : wellscoped_type (Tqualified q t)
+  | wellscoped_loc_info {li t} (_ : wellscoped_type t)
+    : wellscoped_type (TLocInfo li t)
   | wellscoped_array t n
     (_ : (n <> 0)%N) : (* From Krebbers. Probably needed to reject [T[][]]. *)
     wellscoped_type t ->
@@ -774,9 +788,9 @@ Combined Scheme complete_mut_ind from complete_decl_mut_ind, complete_basic_type
   wellscoped_type_mut_ind, wellscoped_types_mut_ind.
 
 Lemma complete_basic_type_not_ref te t : complete_basic_type te t → not_ref_type t.
-Proof. by inversion 1. Qed.
+Proof. induction 1; cbn; auto. Qed.
 Lemma complete_pointee_type_not_ref te t : complete_pointee_type te t → not_ref_type t.
-Proof. induction 1; by [eapply complete_basic_type_not_ref | ]. Qed.
+Proof. induction 1; cbn; eauto using complete_basic_type_not_ref. Qed.
 
 Lemma complete_type_not_ref_ref te t1 t2 : complete_type te t1 → ref_to_type t1 = Some t2 → not_ref_type t2.
 Proof.
